Changed the axioms of transient: it now takes two parameters
This makes a cleaner separation between syntax and semantics

unity/logic.lean
@@ -7,7 +7,7 @@ import unity.safety
 
 import util.logic
 
-universe variables u
+universe variables u v
 
 namespace unity
 
@@ -16,62 +16,136 @@ section connectors
 open predicate
 
 class system (α : Type u) extends has_safety α : Type (u+1) :=
-   (transient : α → pred' σ → Prop)
+   (transient : α → pred' σ → pred' σ → Prop)
    (init : α → pred' σ → Prop)
-   (transient_false : ∀ s : α, transient s $ λ _, false)
-   (transient_str : ∀ (s : α) {p q : σ → Prop},
-         (∀ i, p i → q i) →
-         transient s q →
-         transient s p )
+   (transient_false : ∀ {s} (p : pred' σ), transient s p False)
+   (transient_antimono : ∀ {s : α} {p q p' q' : pred' σ},
+         (p' ⟹ p) →
+         (q' ⟹ q) →
+         transient s p q →
+         transient s p' q' )
 
-def system.state (α : Type u) [system α] := has_safety.σ α
+parameters (α : Type u) [system α] (s : α)
 
-def transient {α} [system α] (s : α) (p : pred' (state α)) : Prop
-:= system.transient s p
+def system.state := has_safety.σ α
 
-def init {α} [system α] (s : α) (p : pred' (state α)) : Prop
+parameters {α}
+
+def transient (p : pred' (state α)) : Prop
+:= system.transient s True p
+
+def transient' (p q : pred' (state α)) : Prop
+:= system.transient s p q
+
+
+lemma system.transient_str {p q r : pred' (state α)}
+  (H : r ⟹ q)
+: transient' p q → transient' p r :=
+system.transient_antimono (by refl) H
+
+def init (p : pred' (state α)) : Prop
 := system.init s p
 
-inductive leads_to {α} [system α] (s : α) : pred' (state α) → pred' (state α) → Prop
-  | basis : ∀ {p q},
-          transient s (p && - q) →
+inductive leads_to : pred' (state α) → pred' (state α) → Prop
+  | trivial {} : ∀ {p}, leads_to p True
+  | basis' : ∀ {p q : pred' (state α)} r,
+          transient' r (p && - q) →
           unless s p q →
+          leads_to (p && -q) (r || q) →
           leads_to p q
   | trans : ∀ {p} q {r}, leads_to p q → leads_to q r → leads_to p r
   | disj : ∀ (t : Type) (p : t → pred' (state α)) {q},
          (∀ i, leads_to (p i) q) →
          leads_to (∃∃ i, p i) q
 
+local notation x ` ↦ `:60 y ` in ` s := leads_to x y
+
+inductive often_imp_often : pred' (state α) → pred' (state α) → Prop
+  | transient : ∀ {p q}, transient' p (-q) → often_imp_often p q
+  | trans : ∀ {p} q {r}, often_imp_often p q → often_imp_often q r → often_imp_often p r
+  | induct : ∀ (t : Type) (V : state α → t) (lt : t → t → Prop)
+         (wf : well_founded lt)
+         {p q}
+         (P : ∀ v, p && eq v ∘ V  ↦  flip lt v ∘ V || q  in  s)
+         (S : ∀ v, unless s (eq v ∘ V) (flip lt v ∘ V || q)),
+         often_imp_often p q
+
 end connectors
 
-notation x ` ↦ `:60 y ` in ` s := leads_to s x y
+notation x `  ↦  `:60 y ` in ` s := leads_to s x y
+notation x `  >~>  `:60 y ` in ` s := often_imp_often s x y
+
+section conversion
+
+parameter {α  : Type u}
+parameter {α' : Type v}
+parameter [system α]
+parameter [system α']
+parameter (f : state α' → state α)
+parameters (s : α) (s' : α')
+parameter (Tf : ∀ {p q}, transient' s p q → transient' s' (p ∘ f) (q ∘ f))
+parameter (Uf : ∀ {p q}, unless s p q → unless s' (p ∘ f) (q ∘ f))
+
+include Tf Uf
+
+lemma leads_to.subst : ∀ {p q}
+  (H : p ↦ q in s),
+  (p ∘ f) ↦ (q ∘ f) in s' :=
+begin
+  apply leads_to.drec,
+  { intro p, apply leads_to.trivial },
+  { intros p q b t u P₀ P₁,
+    apply leads_to.basis' (b ∘ f),
+    { apply Tf t },
+    { apply Uf u },
+    { apply P₁ }, },
+  { intros p q r Pa₀ Pa₁ Pb₀ Pb₁,
+    apply leads_to.trans (q ∘ f) Pb₀ Pb₁, },
+  { intros t p q Pa Pb,
+    apply leads_to.disj t _ Pb },
+end
+
+lemma often_imp_often.subst : ∀ {p q}
+  (H : p >~> q in s),
+  (p ∘ f) >~> (q ∘ f) in s' :=
+begin
+  apply often_imp_often.drec,
+  { intros p q T,
+    apply often_imp_often.transient (Tf T) },
+  { intros p q r _ _ Pb₀ Pb₁,
+    apply often_imp_often.trans _ Pb₀ Pb₁ },
+  { intros t V lt wf p q P S,
+    apply often_imp_often.induct t (V ∘ f) lt wf,
+    { intro v, apply leads_to.subst f s s' @Tf @Uf (P v), },
+    { intro v, apply Uf (S v) } },
+end
+
+end conversion
 
 open predicate
 
-theorem system.unless_conj {α} [system α] (s : α) {p₀ q₀ p₁ q₁ : pred' (state α)} :
-         unless s p₀ q₀ →
-         unless s p₁ q₁ →
-         unless s (p₀ && p₁) (q₀ || q₁) :=
+section rules
+
+parameters {α : Type u} [system α]
+parameter {s : α}
+
+lemma leads_to.basis {p q : pred' (state α)}
+  (h₀ : transient s (p && - q))
+  (h₁ : unless s p q)
+: leads_to s p q :=
 begin
-  intros h₀ h₁,
-  note h₂ := unless_conj_gen _ h₀ h₁,
-  apply unless_weak_rhs _ _ h₂,
-  intros i,
-  unfold p_and p_or, intro h,
-  cases h with h h,
-  cases h with h h,
-  { cases h with h₂ h₃, exact or.inl h₂ },
-  { cases h with h₂ h₃, exact or.inr h₃ },
-  { cases h with h₂ h₃, exact or.inl h₂ },
+  apply leads_to.basis' _ h₀ h₁,
+  rw True_p_or, apply leads_to.trivial
 end
 
+parameter s
 
-theorem leads_to.impl {α} [system α] (s : α) {p q : pred' (state α)}
+theorem leads_to.impl {p q : pred' (state α)}
    (h : p ⟹ q)
    : p ↦ q in s :=
 begin
   apply leads_to.basis,
-  { assert h' : (p && -q) = λ _, false,
+  { assert h' : (p && -q) = False,
     { apply funext,
       intro x, unfold p_and p_not,
       apply eq_false_of_not_eq_true,
@@ -83,9 +157,9 @@ begin
   apply impl_unless _ h
 end
 
-open predicate
+parameter {s}
 
-theorem leads_to.weaken_lhs {α} [system α] {s : α} (q : pred' (state α)) {p r : pred' (state α)}
+theorem leads_to.weaken_lhs (q : pred' (state α)) {p r : pred' (state α)}
     (H  : p ⟹ q)
     (P₀ : q  ↦ r in s)
     : p ↦ r in s :=
@@ -95,7 +169,7 @@ begin
   apply P₀
 end
 
-theorem leads_to.strengthen_rhs {α} [system α] {s : α}
+theorem leads_to.strengthen_rhs
     (q : pred' (state α)) {p r : pred' (state α)}
     (H  : q ⟹ r)
     (P₀ : p  ↦ q in s)
@@ -106,7 +180,18 @@ begin
   apply leads_to.impl s H,
 end
 
-lemma leads_to.disj_rng {α} [system α] {s : α} {t : Type} {p : t → pred' (state α)} {q} {r : t → Prop}
+theorem leads_to.monotonicity
+  {p p' q q' : pred' (state α)}
+  (Hp : p' ⟹ p)
+  (Hq : q  ⟹ q')
+  (P₀ : p  ↦ q in s)
+: p' ↦ q' in s :=
+begin
+  apply leads_to.weaken_lhs _ Hp,
+  apply leads_to.strengthen_rhs _ Hq P₀,
+end
+
+lemma leads_to.disj_rng {t : Type} {p : t → pred' (state α)} {q} {r : t → Prop}
          (h : ∀ i, r i → p i ↦ q in s)
          : (∃∃ i, (λ _, r i) && p i) ↦ q in s :=
 begin
@@ -125,19 +210,19 @@ begin
   apply i^.property
 end
 
-theorem leads_to.disj' {α} [system α] {s : α} {p q r : pred' (state α)}
+theorem leads_to.disj' {p q r : pred' (state α)}
     (Pp : p ↦ r in s)
     (Pq : q ↦ r in s)
     : p || q ↦ r in s :=
 begin
-  apply leads_to.weaken_lhs (λ i, (∃ x : bool, (if x then p else q) i)),
+  apply leads_to.weaken_lhs (∃∃ x : bool, (if x then p else q)),
   { intro i,
-    apply or.rec,
+    apply or.rec ; unfold p_exists,
     { intro h,
       existsi tt, apply h },
     { intro h,
       existsi ff, apply h }, },
-  { apply @leads_to.disj _ _ _ bool (λ (x : bool) i, (if x then p else q) i),
+  { apply @leads_to.disj _ _ _ bool,
     intro i,
     cases i,
     { refine leads_to.weaken_lhs _ _ Pq,
@@ -180,9 +265,7 @@ begin
   intro, apply id
 end
 
-def rel α [system α] : Type := system.state α → system.state α → Prop
-
-theorem leads_to.induction' {α} {β : Type} [system α] {s : α} {lt' : β → β → Prop}
+theorem leads_to.induction' {β : Type} {lt' : β → β → Prop}
     (wf : well_founded lt')
     (V : state α → β)
     {p q : pred' (state α)}
@@ -191,7 +274,7 @@ theorem leads_to.induction' {α} {β : Type} [system α] {s : α} {lt' : β → 
 begin
   pose lt := flip lt',
   assert P' : (∃∃ v, p && eq v ∘ V)  ↦ q in s,
-  { apply leads_to.disj β (λ v, p && eq v ∘ V), intro i,
+  { apply leads_to.disj β, intro i,
     pose PP := λ i, p && eq i ∘ V  ↦  q in s,
     change PP i,
     apply @well_founded.induction _ lt' wf PP,
@@ -222,25 +305,35 @@ begin
     apply P' }
 end
 
-theorem leads_to.induction {α} [system α] {s : α} {lt' : rel α} (wf : well_founded lt')
+def rel : Type := system.state α → system.state α → Prop
+
+theorem leads_to.induction {lt' : rel} (wf : well_founded lt')
     {p q : pred' (state α)}
     (P : ∀ v, p && eq v  ↦ p && flip lt' v || q in s)
   : p ↦ q in s :=
-leads_to.induction' wf id P
+leads_to.induction' wf _ P
 
-theorem leads_to.PSP {α} [system α] {s : α} {p q r b : pred' (state α)}
+theorem leads_to.PSP {p q r b : pred' (state α)}
     (P : p ↦ q in s)
     (S : unless s r b)
     : p && r  ↦  (q && r) || b in s :=
 begin
-  induction P with p₀ q₀ t₀ u₀ p₁ q₁ r₁ PP₀ PP₁,
-  { apply leads_to.basis,
-    { apply system.transient_str _ _ t₀, intro i,
-      simp, intro h,
-      cases h with h h', cases h' with h₀ h₁,
-      split, assumption,
-      intro h₂, apply h₁, apply or.inr,
-      split, assumption, assumption, },
+  induction P with b p₀ q₀ b₀ t₀ u₀ P PSP₀
+         p₁ q₁ r₁ PP₀ PP₁,
+  { apply leads_to.impl,
+    apply p_and_entails_of_entails_right,
+    apply entails_p_or_of_entails_left,
+    simp, },
+  { apply leads_to.basis' b₀,
+    { apply system.transient_str _ _ t₀,
+      apply entails_p_and_of_entails,
+      { apply p_and_entails_of_entails_left,
+        simp },
+      { rw [p_not_p_or,p_not_p_and,p_and_assoc],
+        apply p_and_entails_of_entails_left _,
+        rw -p_and_assoc,
+        apply p_and_entails_of_entails_right _,
+        rw p_and_p_or_p_not_self, simp } },
     { assert H : unless s r (r || b),
       { apply impl_unless, intro, apply or.inl },
       assert H' : unless s p₀ (q₀ || b),
@@ -252,7 +345,29 @@ begin
       intro hh, cases hh with hh₀ hh₀, cases hh₀ with hh₀ hh₀,
       { cases hh₀ with hh₀ hh₁, exact or.inl ⟨hh₀,hh₁⟩ },
       { cases hh₀ with hh₀ hh₁, exact or.inr hh₁ },
-      { cases hh₀ with hh₀ hh₁, exact or.inr hh₁ } } },
+      { cases hh₀ with hh₀ hh₁, exact or.inr hh₁ } },
+    { apply leads_to.monotonicity _ _ PSP₀,
+      { apply entails_p_and_of_entails,
+        apply entails_p_and_of_entails,
+        { apply p_and_entails_of_entails_left,
+          apply p_and_elim_left },
+        { rw [p_not_p_or,p_not_p_and,p_and_assoc],
+          apply p_and_entails_of_entails_left _,
+          rw [-p_and_assoc],
+          apply p_and_entails_of_entails_right _,
+          rw [p_and_p_or_p_not_self],
+          apply p_and_elim_right _ _, },
+        { apply p_and_entails_of_entails_left,
+          apply p_and_elim_right } },
+      { apply p_or_entails_of_entails,
+        { rw p_and_over_or_right,
+          apply p_or_entails_of_entails,
+          apply entails_p_or_of_entails_left,
+          { apply p_and_elim_left },
+          { apply entails_p_or_of_entails_right,
+            apply p_or_intro_left }, },
+        { apply entails_p_or_of_entails_right,
+          apply p_or_intro_right } }, } },
   { note H := leads_to.cancellation _ ih_1 ih_2,
     assert H' : (r₁ && r || b || b) = (r₁ && r || b),
     { apply funext, intro,
@@ -267,29 +382,9 @@ begin
     apply ih_1 i, },
 end
 
-lemma True_leads_to_True {α} [system α] (s : α)
+lemma True_leads_to_True
 : True ↦ True in s :=
-begin
-  apply leads_to.basis,
-  { assert H : (True && -True) = (False : pred' (state α)),
-    { apply funext, intro x, simp },
-    rw H,
-    apply system.transient_false },
-  { apply True_unless }
-end
-
-inductive often_imp_often {α} [system α] (s : α) : pred' (state α) → pred' (state α) → Prop
-  | trans : ∀ {p} q {r}, often_imp_often p q → often_imp_often q r → often_imp_often p r
-  | induct : ∀ (t : Type) (V : state α → t) (lt : t → t → Prop)
-         (wf : well_founded lt)
-         {p q}
-         (P : ∀ v, p && eq v ∘ V  ↦  flip lt v ∘ V || q  in  s)
-         (S : ∀ v, unless s (eq v ∘ V) (flip lt v ∘ V || q)),
-         often_imp_often p q
-
-section lemmas
-
-parameters {α : Type u} [system α] (s : α)
+leads_to.trivial
 
 lemma often_imp_often.basis {p q}
           (h : p ↦ q in s)
@@ -305,12 +400,12 @@ begin
   ; intro,
   { rw [H,False_p_or],
     apply leads_to.weaken_lhs _ _ h,
-    apply p_and_left, },
+    apply p_and_elim_left, },
   { rw [H'],
     apply True_unless }
 end
 
-end lemmas
+end rules
 
 open predicate
 
@@ -322,10 +417,10 @@ class system_sem (α : Type u) extends system α :=
          ex s τ →
          init s p →
          (•p) τ)
-  (transient_sem : ∀ {s : α} {p : pred' _} (τ : stream _),
+  (transient_sem : ∀ {s : α} {p q : pred' _} (τ : stream _),
          ex s τ →
-         transient s p →
-         ([]<>-•p) τ)
+         transient' s p q →
+         ([]<>•p) τ → ([]<>-•q) τ)
 
 namespace system_sem
 
@@ -344,14 +439,30 @@ lemma leads_to_sem {s : α} {p q : pred' (state α)}
 : (•p ~> •q) τ :=
 begin
   note saf : saf_ex s τ := system_sem.safety s _ sem,
-  induction P with p' q' T S
+  induction P with
+        p'
+        p q b T S B Bsem
         p q r P₀ P₁ H₀ H₁
         X p q P₀ H₀ x y z,
+    -- trivial
+  { apply temporal.leads_to_of_inf_often,
+    simp, },
     -- transient and unless
   { intros i hp,
     note saf' := unless_sem' _ _ saf S (temporal.eventually_weaken _ hp),
     cases saf' with saf' saf',
-    { note T' := transient_sem τ sem T,
+    { assert T' : ([]<>-•(p && -q)) τ,
+      { rw [-or_self (([]<>-•(p && -q)) τ),or_iff_not_imp],
+        rw [p_not_eq_not,not_henceforth,not_eventually,p_not_p_not_iff_self],
+        apply function.comp _ (inf_often_of_stable _),
+        intro H,
+        rw [-or_self (([]<>-•(p && -q)) τ)],
+        apply or.imp_left (transient_sem τ sem T),
+        rw [-p_or_to_fun,-inf_often_p_or],
+        rw [not_init,p_not_p_and,p_not_p_not_iff_self,-init_p_or],
+        apply inf_often_entails_inf_often' _ _ (inf_often_of_leads_to Bsem H),
+        { apply p_or_entails_p_or_right,
+          apply p_or_intro_right, }, },
       note T'' := (coincidence saf' (henceforth_drop i T')),
       apply eventually_entails_eventually _ _ (henceforth_str _ T''),
       intros τ',
@@ -379,21 +490,24 @@ lemma often_imp_often_sem'
      (sem : ex s τ)
 : ∀ {p q : pred' (state α)} (P : often_imp_often s p q),
     ([]<>•p ⟶ []<>•q) τ :=
-  @often_imp_often.drec α _ s _
-      (take p q r P₀ P₁,
-       assume Lpq : ([]<>•p ⟶ []<>•q) τ,
-       assume Lqr : ([]<>•q ⟶ []<>•r) τ,
-       assume Hp : ([]<>•p) τ,
-       show ([]<>•r) τ, from Lqr (Lpq Hp))
-      begin
-        intros t V lt wf p q P₀ S₀,
-        apply inf_often_induction' V p q wf,
-        { intro v,
-          apply unless_sem_str _ _ (S₀ v),
-          apply system_sem.safety _ _ sem, },
-        { intro v,
-          apply leads_to_sem (P₀ v) _ sem, }
-      end
+begin
+  apply @often_imp_often.drec α _ s _ _ _ _,
+  { intros p q T,
+    note Tsem : ([]<>•p ⟶ []<>-•-q) τ
+              := system_sem.transient_sem _ sem T,
+    rw [not_init,p_not_p_not_iff_self] at Tsem,
+    apply Tsem },
+  { intros p q r P₀ P₁,
+    intros Lpq Lqr Hp,
+    show ([]<>•r) τ, from Lqr (Lpq Hp) },
+  { intros t V lt wf p q P₀ S₀,
+    apply inf_often_induction' V p q wf,
+    { intro v,
+      apply unless_sem_str _ _ (S₀ v),
+      apply system_sem.safety _ _ sem, },
+    { intro v,
+      apply leads_to_sem (P₀ v) _ sem, } }
+end
 
 end
 
