unity/models/det.lean
@@ -34,42 +34,40 @@ s^.take_step e σ = σ'
 def is_step (s : program lbl α) (σ σ' : α) : Prop :=
 ∃ ev, s.action_of ev σ σ'
 
-def program.falsify (s : program lbl α) (ev : option lbl) (p : pred α) : Prop
-:= ∀ σ, p σ → ¬ (p (s^.take_step ev σ))
+def program.falsify (s : program lbl α) (ev : option lbl) (p q : pred α) : Prop :=
+∀ σ, q σ → ¬ (q (s^.take_step ev σ))
 
-def program.transient (s : program lbl α) (p : pred α) : Prop
-:= ∃ ev, s.falsify ev p
+def program.transient (s : program lbl α) (p q : pred α) : Prop
+:= ∃ ev, s.falsify ev p q
 
-def program.falsify_action (s : program lbl α) (p : pred α) (ev : option lbl)
-  (h : s.falsify ev p)
-: •p ⟹ ( ⟦ s.action_of ev ⟧ ⟶ ⟦ λ _, - p ⟧ ) :=
+def program.falsify_action (s : program lbl α) (p q : pred α) (ev : option lbl)
+  (h : s.falsify ev p q)
+: •q ⟹ ( ⟦ s.action_of ev ⟧ ⟶ ⟦ λ _, - q ⟧ ) :=
 begin
   unfold program.transient at h,
-  intros τ H₀ H₁,
+  intros τ Hq H₁,
   unfold temporal.action program.action_of at H₁,
   unfold temporal.action,
   rw -H₁,
-  apply h,
-  apply H₀
+  apply (h _ Hq),
 end
 
 lemma program.falsify.negate
-   {s : program lbl α} {act : option lbl} {p : pred' α}
-:  s.falsify act p
-→  •p && ⟦ s^.action_of act ⟧ ⟹ <>-•p :=
+   {s : program lbl α} {act : option lbl} {p q : pred' α}
+:  s.falsify act p q
+→  •q && ⟦ s^.action_of act ⟧ ⟹ <>-•q :=
 begin
   intros FALSE τ H,
-  assert GOAL : ⟦ λ _, - p ⟧ τ,
+  assert GOAL : ⟦ λ _, - q ⟧ τ,
   { cases H with H₀ H₁,
-    apply s.falsify_action p act FALSE
-    ; assumption },
+    apply s.falsify_action p q act FALSE _ H₀ H₁, },
   unfold temporal.eventually,
   existsi 1,
   apply GOAL
 end
 
-lemma program.transient_false (s : program lbl α) 
-: s.transient False :=
+lemma program.transient_impl (s : program lbl α) (p : pred' α)
+: s.transient p False :=
 begin
   unfold program.transient False,
   existsi @none lbl,
@@ -77,18 +75,18 @@ begin
   cases h
 end
 
-lemma program.transient_str (s : program lbl α) (p q : α → Prop)
-  (h : ∀ (i : α), p i → q i)
-  (T₀ : s.transient q)
-: s.transient p :=
+lemma program.transient_antimono (s : program lbl α) {p q p' q' : α → Prop}
+  (hp : p' ⟹ p)
+  (hq : q' ⟹ q)
+  (T₀ : s.transient p q)
+: s.transient p' q' :=
 begin
   unfold program.transient,
   cases T₀ with ev T₁,
   existsi ev,
-  intros σ h',
-  note h'' := T₁ σ (h _ h'),
-  intro h₂, apply h'',
-  apply h _ h₂
+  intros σ,
+  apply imp_mono (hq _) _ (T₁ σ),
+  apply contrapos (hq _),
 end
 
 instance prog_is_system : unity.system (program lbl α) :=
@@ -96,8 +94,8 @@ instance prog_is_system : unity.system (program lbl α) :=
   , init := program.init
   , step := is_step
   , transient := program.transient
-  , transient_false := program.transient_false
-  , transient_str := program.transient_str
+  , transient_false := λ s p, program.transient_impl s _
+  , transient_antimono := program.transient_antimono
   }
 
 open temporal
@@ -117,7 +115,7 @@ def run (s : program lbl α) (τ : stream (option lbl)) : stream α
 
 section soundness
 
-variables {s : program lbl α} {p : pred' α}
+variables {s : program lbl α} {p q : pred' α}
 variables (τ : stream α)
 variables h : ex s τ
 include h
@@ -133,18 +131,19 @@ begin
 end
 
 lemma transient.semantics
-  (T₀ : s.transient p)
-: ([]<>-•p) τ :=
+  (T₀ : s.transient p q)
+: ([]<>•p) τ → ([]<>-•q) τ :=
 begin
+  intro,
   unfold program.transient at T₀,
   cases T₀ with ev T₀,
-  cases temporal.em' (• p) τ with hp hnp,
-  { note occ := coincidence hp (h.liveness ev),
+  cases temporal.em' (• q) τ with hq hnq,
+  { note occ := coincidence hq (h.liveness ev),
     rw -eventually_eventually,
     apply henceforth_entails_henceforth _ _ occ,
     apply eventually_entails_eventually,
     apply T₀.negate },
-  { apply hnp }
+  { apply hnq }
 end
 
 end soundness
@@ -182,6 +181,6 @@ instance {α} [sched lbl] : system_sem (program lbl α) :=
   , safety := @ex.safety _ _
   , inhabited := program.witness
   , init_sem := @init_sem _ _
-  , transient_sem := @transient.semantics _ _ }
+  , transient_sem := @transient.semantics _ _  }
 
 end det
