unity/models/simple.lean
@@ -21,30 +21,32 @@ def False {α} : pred α := λ_, false
 def program.init {α} (s : program α) (p : pred α) : Prop
 := p (s^.first)
 
-def program.transient {α} (s : program α) (p : pred α) : Prop
-:= ∀ σ, p σ → ¬ (p (s^.step σ))
+def program.transient {α} (s : program α) (p q : pred α) : Prop
+:= ∀ σ, p σ → q σ → ¬ (q (s^.step σ))
 
 def program.unless {α} (s : program α) (p q : pred α) : Prop
 := ∀ σ, p σ ∧ ¬q σ → p (s^.step σ) ∨ q (s^.step σ)
 
-lemma program.transient_false {α} (s : program α)
-: s.transient False :=
-begin
-  unfold program.transient False,
-  intros σ h,
-  cases h
-end
-
-lemma program.transient_str {α} (s : program α) (p q : α → Prop)
-  (h : ∀ (i : α), p i → q i)
-  (T₀ : s.transient q)
-: s.transient p :=
+lemma program.transient_impl {α} (s : program α) {p q : α → Prop}
+  (H : p ⟹ -q)
+: s.transient p q :=
 begin
   unfold program.transient,
-  intros σ h',
-  note h'' := T₀ σ (h _ h'),
+  intros σ hp hq,
+  cases H _ hp hq,
+end
+
+lemma program.transient_antimono {α} (s : program α) (p q p' q' : α → Prop)
+  (hp : p' ⟹ p)
+  (hq : q' ⟹ q)
+  (T₀ : s.transient p q)
+: s.transient p' q' :=
+begin
+  unfold program.transient,
+  intros σ hp' hq',
+  note h'' := T₀ σ (hp _ hp') (hq _ hq'),
   intro h₂, apply h'',
-  apply h _ h₂
+  apply hq _ h₂
 end
 
 def is_step {α} (s : program α) (σ σ' : α) : Prop := σ' = s.step σ
@@ -54,8 +56,8 @@ instance prog_is_system {α} : system (program α) :=
   , step := is_step
   , init := program.init
   , transient := program.transient
-  , transient_false := program.transient_false
-  , transient_str := program.transient_str
+  , transient_false := λ s p, program.transient_impl s (by simp)
+  , transient_antimono := program.transient_antimono
   }
 
 lemma unless_step {α : Type}
@@ -84,7 +86,7 @@ lemma leads_to_step {α : Type}
 begin
   apply leads_to.basis,
   { unfold transient system.transient program.transient program.step,
-    intros σ h,
+    intros σ _ h,
     cases h with h₀ h₁,
     note h' := h _ h₀ h₁,
     simp [not_and_iff_not_or_not,not_not_iff_self],
@@ -96,19 +98,31 @@ end
 
 open nat
 
-def ex {α} (s : program α) : stream α
-  | 0 := s^.first
-  | (succ n) := s^.step $ ex n
+open temporal
+
+def ex {α} (s : program α) : cpred α :=
+•eq s.first && [] ⟦ is_step s ⟧
 
 lemma ex.safety {α} {s : program α} (τ : stream α)
-  (h : τ = ex s)
-: ∀ i, ⟦ is_step s ⟧ (τ.drop i) :=
+  (h : ex s τ)
+: [] ⟦ is_step s ⟧ $ τ :=
+h.right
+
+def ex.witness {α} (s : program α) : stream α
+  | 0 := s.first
+  | (succ i) := s.step (ex.witness i)
+
+lemma ex.witness_correct  {α} (s : program α)
+: ex s (ex.witness s) :=
 begin
-  intro i,
-  subst τ,
-  unfold temporal.action is_step stream.drop,
-  simp [add_one_eq_succ],
-  refl
+  unfold ex, simp,
+  split,
+  { intro i,
+    rw action_drop,
+    unfold is_step,
+    refl },
+  { unfold temporal.init,
+    refl }
 end
 
 section semantics
@@ -117,9 +131,10 @@ universe variable u
 
 parameter {α : Type}
 variable {s : program α}
-variable {p : pred α}
+variables {p q : pred α}
 variable τ : stream α
-variable (H : τ = ex s)
+variable (H : ex s τ)
+open temporal
 
 include H
 
@@ -129,33 +144,41 @@ lemma init_sem
 begin
   unfold init system.init program.init at I₀,
   unfold temporal.init,
-  rw H, apply I₀,
+  note H' := H.left,
+  unfold temporal.init at H',
+  rw -H', apply I₀,
 end
 
 lemma transient.semantics
-  (T₀ : transient s p)
-: ([]<>-•p) τ :=
+  (T₀ : transient' s p q)
+: ([]<>•p) τ → ([]<>•-q) τ :=
 begin
-  intros i,
-  cases classical.em ((•p) (stream.drop i τ)) with hp hnp,
-  { unfold transient system.transient program.transient at T₀,
-    unfold temporal.eventually, existsi 1,
-    subst τ,
-    simp [temporal.not_init,stream.drop_drop],
-    unfold ex p_not temporal.init,
-    apply T₀ _ hp, },
-  { unfold temporal.eventually p_not, existsi 0,
-    simp [stream.drop_drop],
-    apply hnp },
+  intros Hp,
+  assert Hstep : (<>[]⟦is_step s⟧) τ,
+  { apply eventually_weaken,
+    apply ex.safety τ H },
+  note H' := coincidence Hstep Hp,
+  rw -eventually_eventually,
+  apply inf_often_entails_inf_often _ _ H',
+  { unfold p_entails, rw p_and_p_imp,
+    intros τ Hs Hp,
+    cases classical.em (•q $ τ) with Hq Hnq,
+    { apply eventually_of_next,
+      unfold transient' system.transient program.transient at T₀,
+      unfold action is_step at Hs,
+      rw [next_init,Hs],
+      apply T₀ _ Hp Hq, },
+    { rw [-p_not_to_fun,not_init] at Hnq,
+      apply eventually_weaken _ Hnq }, },
 end
 
 end semantics
 
 instance {α} : system_sem (program α) :=
   { (_ : system (program α)) with
-    ex := λ p τ, τ = ex p
+    ex := ex
   , safety := @ex.safety _
-  , inhabited := λ p, ⟨ex p, rfl⟩
+  , inhabited := λ p, ⟨ex.witness p, ex.witness_correct p⟩
   , init_sem := @init_sem _
   , transient_sem := @transient.semantics _ }
 
